Internal Layout Polishing

examples/technical_report/TR_my_commented_isabelle/TR_MyCommentedIsabelle.thy
@@ -18,43 +18,43 @@ text*[bu::author,
 text*[abs::abstract,
       keywordlist="[''LCF-Architecture'',''Isabelle'',''SML'',''PIDE'',''Programming Guide'',
                     ''Tactic Programming'']"]\<open>
-While Isabelle is mostly known as part of Isabelle/HOL (an interactive 
-theorem prover), it actually provides a system framework for developing a wide
-spectrum of applications. A particular strength of the Isabelle framework is the 
-combination of text editing, formal verification, and code generation. 
-
-This is a programming-tutorial of Isabelle and Isabelle/HOL, a complementary
-text to the unfortunately somewhat outdated "The Isabelle Cookbook" in
-\url{https://nms.kcl.ac.uk/christian.urban/Cookbook/}. The reader is encouraged
-not only to consider the generated .pdf, but also consult the loadable version in Isabelle/jEdit
-@{cite "DBLP:journals/corr/Wenzel14"}in order to make experiments on the running code.
-
-This text is written itself in Isabelle/Isar using a specific document ontology
-for technical reports. It is intended to be a "living document", i.e. it is not only
-used for generating a static, conventional .pdf, but also for direct interactive 
-exploration in Isabelle/jedit. This way, types, intermediate results of computations and
-checks can be repeated by the reader who is invited to interact with this document.
-Moreover, the textual parts have been enriched with a maximum of formal content
-which makes this text re-checkable at each load and easier maintainable.
+  While Isabelle is mostly known as part of Isabelle/HOL (an interactive 
+  theorem prover), it actually provides a system framework for developing a wide
+  spectrum of applications. A particular strength of the Isabelle framework is the 
+  combination of text editing, formal verification, and code generation. 
+  
+  This is a programming-tutorial of Isabelle and Isabelle/HOL, a complementary
+  text to the unfortunately somewhat outdated "The Isabelle Cookbook" in
+  \url{https://nms.kcl.ac.uk/christian.urban/Cookbook/}. The reader is encouraged
+  not only to consider the generated .pdf, but also consult the loadable version in Isabelle/jEdit
+  @{cite "DBLP:journals/corr/Wenzel14"}in order to make experiments on the running code.
+  
+  This text is written itself in Isabelle/Isar using a specific document ontology
+  for technical reports. It is intended to be a "living document", i.e. it is not only
+  used for generating a static, conventional .pdf, but also for direct interactive 
+  exploration in Isabelle/jedit. This way, types, intermediate results of computations and
+  checks can be repeated by the reader who is invited to interact with this document.
+  Moreover, the textual parts have been enriched with a maximum of formal content
+  which makes this text re-checkable at each load and easier maintainable.
 \<close>
 
 chapter*[intro::introduction]\<open> Introduction  \<close>    
 
-text\<open>
-While Isabelle @{cite "DBLP:books/sp/NipkowPW02"} is mostly known as part of Isabelle/HOL (an interactive theorem prover), it actually 
-provides a system framework for developing a wide spectrum of applications. A particular strength of 
-the Isabelle framework is the combination of text editing, formal verification, and code generation.
-This is a programming-tutorial of Isabelle and Isabelle/HOL, a complementary text to the 
-unfortunately somewhat outdated "The Isabelle Cookbook" in 
-\url{https://nms.kcl.ac.uk/christian.urban/Cookbook/}. The reader is encouraged not only to consider 
-the generated .pdf, but also consult the loadable version in Isabelle/jedit in order to make 
-experiments on the running code. This text is written itself in Isabelle/Isar using a specific 
-document ontology for technical reports. It is intended to be a "living document", i.e. it is not 
-only used for generating a static, conventional .pdf, but also for direct interactive exploration 
-in Isabelle/jedit. This way, types, intermediate results of computations and checks can be 
-repeated by the reader who is invited to interact with this document. Moreover, the textual 
-parts have been enriched with a maximum of formal content which makes this text re-checkable at 
-each load and easier maintainable.\<close>
+text\<open> While Isabelle @{cite "DBLP:books/sp/NipkowPW02"} is mostly known as part of Isabelle/HOL 
+  (an interactive theorem prover), it actually provides a system framework for developing a wide 
+  spectrum of applications. A particular strength of the Isabelle framework is the combination 
+  of text editing, formal verification, and code generation. This is a programming-tutorial of 
+  Isabelle and Isabelle/HOL, a complementary text to the unfortunately somewhat outdated 
+  "The Isabelle Cookbook" in \url{https://nms.kcl.ac.uk/christian.urban/Cookbook/}. The reader 
+  is encouraged not only to consider the generated .pdf, but also consult the loadable version 
+  in Isabelle/jedit in order to make experiments on the running code. This text is written 
+  itself in Isabelle/Isar using a specific document ontology for technical reports. It is 
+  intended to be a "living document", i.e. it is not only used for generating a static, 
+  conventional .pdf, but also for direct interactive exploration in Isabelle/jedit. This way, 
+  types, intermediate results of computations and checks can be repeated by the reader who is 
+  invited to interact with this document. Moreover, the textual parts have been enriched with a 
+  maximum of formal content which makes this text re-checkable at each load and easier 
+  maintainable.\<close>
 
 figure*[architecture::figure,relative_width="80",src="''figures/isabelle-architecture''"]\<open> 
      The system architecture of Isabelle (left-hand side) and the 
@@ -62,10 +62,10 @@ figure*[architecture::figure,relative_width="80",src="''figures/isabelle-archite
      the IDE (right-hand side). \<close>
 
 text\<open>This cookbook roughly follows the Isabelle system architecture shown in 
-@{figure "architecture"}, and, to be more precise, more or less in the bottom-up order.
+  @{figure "architecture"}, and, to be more precise, more or less in the bottom-up order.
 
-We start from the basic underlying SML platform over the Kernels to the tactical layer 
-and end with a discussion over the front-end technologies.
+  We start from the basic underlying SML platform over the Kernels to the tactical layer 
+  and end with a discussion over the front-end technologies.
 \<close>
 
 chapter*[t1::technical]\<open> SML and Fundamental SML libraries  \<close>    
@@ -73,10 +73,10 @@ chapter*[t1::technical]\<open> SML and Fundamental SML libraries  \<close>
 section*[t11::technical] "ML, Text and Antiquotations"
 
 text\<open>Isabelle is written in SML, the "Standard Meta-Language", which is is an impure functional 
-programming language allowing, in principle, mutable variables and side-effects. 
-The following Isabelle/Isar commands allow for accessing the underlying SML interpreter
-of Isabelle directly. In the example, a mutable variable X is declared, defined to 0 and updated; 
-and finally re-evaluated leading to output: \<close>
+  programming language allowing, in principle, mutable variables and side-effects. 
+  The following Isabelle/Isar commands allow for accessing the underlying SML interpreter
+  of Isabelle directly. In the example, a mutable variable X is declared, defined to 0 and updated; 
+  and finally re-evaluated leading to output: \<close>
 
 ML\<open> val X = Unsynchronized.ref 0;
     X:= !X + 1;
@@ -84,10 +84,10 @@ ML\<open> val X = Unsynchronized.ref 0;
   \<close>
 
 text\<open>However, since Isabelle is a platform involving parallel execution, concurrent computing, and,
-as an interactive environment, involves backtracking / re-evaluation as a consequence of user-
-interaction, imperative programming is discouraged and nearly never used in the entire Isabelle
-code-base @{cite "DBLP:conf/mkm/BarrasGHRTWW13"}.
-The preferred programming style is purely functional: \<close>
+  as an interactive environment, involves backtracking / re-evaluation as a consequence of user-
+  interaction, imperative programming is discouraged and nearly never used in the entire Isabelle
+  code-base @{cite "DBLP:conf/mkm/BarrasGHRTWW13"}.
+  The preferred programming style is purely functional: \<close>
 
 ML\<open> fun fac x = if x = 0 then 1 else x * fac(x-1) ;
     fac 10;
@@ -98,20 +98,20 @@ ML\<open> type state = {  a : int,   b : string}
   \<close>
 
 text\<open> The faculty function is defined and executed; the (sub)-interpreter in Isar
-works in the conventional read-execute-print loop for each statement separated by a ";".
-Functions, types, data-types etc. can be grouped to modules (called \<^emph>\<open>structures\<close>) which can
-be constrained to interfaces (called \<^emph>\<open>signatures\<close>) and even be parametric structures
-(called \<^emph>\<open>functors\<close>). \<close>
+  works in the conventional read-execute-print loop for each statement separated by a ";".
+  Functions, types, data-types etc. can be grouped to modules (called \<^emph>\<open>structures\<close>) which can
+  be constrained to interfaces (called \<^emph>\<open>signatures\<close>) and even be parametric structures
+  (called \<^emph>\<open>functors\<close>). \<close>
 
 text\<open> The Isabelle/Isar interpreter (called \<^emph>\<open>toplevel\<close> ) is extensible; by a mixture of SML
-and Isar-commands, domain-specific components can be developed and integrated into the system 
-on the fly. Actually, the Isabelle system code-base consists mainly of SML and \<^verbatim>\<open>.thy\<close>-files 
-containing such mixtures of Isar commands and SML. \<close>
+  and Isar-commands, domain-specific components can be developed and integrated into the system 
+  on the fly. Actually, the Isabelle system code-base consists mainly of SML and \<^verbatim>\<open>.thy\<close>-files 
+  containing such mixtures of Isar commands and SML. \<close>
 
 text\<open> Besides the ML-command used in the above examples, there are a number of commands 
-representing text-elements in Isabelle/Isar; text commands can be interleaved arbitraryly
-with other commands. Text in text-commands may use LaTeX and is used for type-setting 
-documentations in a kind of literate programming style. \<close>
+  representing text-elements in Isabelle/Isar; text commands can be interleaved arbitraryly
+  with other commands. Text in text-commands may use LaTeX and is used for type-setting 
+  documentations in a kind of literate programming style. \<close>
 
 text\<open>So: the text command for:\<close>
 
@@ -127,24 +127,23 @@ figure*[fig2::figure, relative_width="100",src="''figures/text-element''"]
         \<open>A text-element as presented in Isabelle/jedit.\<close>
 
 text\<open> text-commands, ML- commands (and in principle any other command) can be seen as 
-\<^emph>\<open>quotations\<close> over the underlying SML environment (similar to OCaml or Haskell).
-Linking these different sorts of quotations with each other and the underlying SML-envirnment
-is supported via \<^emph>\<open>antiquotations\<close>'s. Generally speaking, antiquotations are a programming 
-technique to specify expressions or patterns in a quotation, parsed in the context of the 
-enclosing expression or pattern where the quotation is. Another way to understand this concept:
-anti-quotations are "semantic macros" that produce a value for the surrounding context
-(ML, text, HOL, whatever) depending on local arguments and the underlying logical context.
-
-The way an antiquotation is specified depends on the quotation expander: typically a specific 
-character and an identifier, or specific parentheses and a complete expression or pattern.\<close>
+  \<^emph>\<open>quotations\<close> over the underlying SML environment (similar to OCaml or Haskell).
+  Linking these different sorts of quotations with each other and the underlying SML-envirnment
+  is supported via \<^emph>\<open>antiquotations\<close>'s. Generally speaking, antiquotations are a programming 
+  technique to specify expressions or patterns in a quotation, parsed in the context of the 
+  enclosing expression or pattern where the quotation is. Another way to understand this concept:
+  anti-quotations are "semantic macros" that produce a value for the surrounding context
+  (ML, text, HOL, whatever) depending on local arguments and the underlying logical context.
+  
+  The way an antiquotation is specified depends on the quotation expander: typically a specific 
+  character and an identifier, or specific parentheses and a complete expression or pattern.\<close>
 
 text\<open> In Isabelle documentations, antiquotation's were heavily used to enrich literate explanations
-and documentations by "formal content", i.e. machine-checked, typed references
-to all sorts of entities in the context of the interpreting environment. 
-Formal content allows for coping with sources that rapidly evolve and were developed by 
-distributed teams as is typical in open-source developments. 
-A paradigmatic example for antiquotation in Texts and Program snippets is here:
-\<close>
+  and documentations by "formal content", i.e. machine-checked, typed references
+  to all sorts of entities in the context of the interpreting environment. 
+  Formal content allows for coping with sources that rapidly evolve and were developed by 
+  distributed teams as is typical in open-source developments. 
+  A paradigmatic example for antiquotation in Texts and Program snippets is here:\<close>
 
 text\<open> @{footnote \<open>sdf\<close>}, @{file "$ISABELLE_HOME/src/Pure/ROOT.ML"}\<close> 
 ML\<open>    val x = @{thm refl};
@@ -155,48 +154,45 @@ ML\<open>    val x = @{thm refl};
 text\<open>... which we will describe in more detail later. \<close> 
 
 text\<open>In a way, literate specification attempting to maximize its formal content is a way to
-ensure "Agile Development" in a (theory)-document development, at least for its objectives, 
-albeit not for its popular methods and processes like SCRUM. \<close>
+  ensure "Agile Development" in a (theory)-document development, at least for its objectives, 
+  albeit not for its popular methods and processes like SCRUM. \<close>
 
 paragraph\<open>
-     A maximum of formal content inside text documentation also ensures the 
-     consistency of this present text with the underlying Isabelle version.\<close>
+  A maximum of formal content inside text documentation also ensures the 
+  consistency of this present text with the underlying Isabelle version.\<close>
 
 section\<open>The Isabelle/Pure bootstrap\<close>
 
 text\<open>It is instructive to study the fundamental bootstrapping sequence of the Isabelle system;
-     it is written in the Isar format and gives an idea of the global module dependencies: 
-     @{file "$ISABELLE_HOME/src/Pure/ROOT.ML"}. Loading this file 
-     (for example by hovering over this hyperlink in the antiquotation holding control or
-     command key in Isabelle/jedit and activating it) allows the Isabelle IDE 
-     to support hyperlinking \<^emph>\<open>inside\<close> the Isabelle source.\<close>
+  it is written in the Isar format and gives an idea of the global module dependencies: 
+  @{file "$ISABELLE_HOME/src/Pure/ROOT.ML"}. Loading this file 
+  (for example by hovering over this hyperlink in the antiquotation holding control or
+  command key in Isabelle/jedit and activating it) allows the Isabelle IDE 
+  to support hyperlinking \<^emph>\<open>inside\<close> the Isabelle source.\<close>
 
-text\<open>The bootstrapping sequence is also reflected in the following diagram
-@{figure "architecture"}.  \<close>
+text\<open>The bootstrapping sequence is also reflected in the following diagram @{figure "architecture"}.\<close>
 
 
 section*[t12::technical] "Elements of the SML library";  
 text\<open>Elements of the @{file "$ISABELLE_HOME/src/Pure/General/basics.ML"} SML library
-are basic exceptions. Note that exceptions should be catched individually, uncatched exceptions 
-except those generated by the specific "error" function are discouraged in Isabelle
-source programming since they might produce races. Finally, a number of commonly
-used "squigglish" combinators is listed:
-\<close>
-ML\<open>
- Bind      : exn;
- Chr       : exn;
- Div       : exn;
- Domain    : exn;
- Fail      : string -> exn;
- Match     : exn;
- Overflow  : exn;
- Size      : exn;
- Span      : exn;
- Subscript : exn;
+  are basic exceptions. Note that exceptions should be catched individually, uncatched exceptions 
+  except those generated by the specific "error" function are discouraged in Isabelle
+  source programming since they might produce races. Finally, a number of commonly
+  used "squigglish" combinators is listed:\<close>
 
- exnName : exn -> string ; (* -- very interesting to query an unknown exception  *)
- exnMessage : exn -> string ;
-\<close>
+ML\<open>   Bind      : exn;
+      Chr       : exn;
+      Div       : exn;
+      Domain    : exn;
+      Fail      : string -> exn;
+      Match     : exn;
+      Overflow  : exn;
+      Size      : exn;
+      Span      : exn;
+      Subscript : exn;
+     
+      exnName : exn -> string ; (* -- very interesting to query an unknown exception  *)
+      exnMessage : exn -> string ;\<close>
 
 ML\<open>
 op ! : 'a Unsynchronized.ref -> 'a;
@@ -215,12 +211,12 @@ K: 'a -> 'b -> 'a
 \<close> 
 
 text\<open>Some basic examples for the programming style using these combinators can be found in the
- "The Isabelle Cookbook" section 2.3.\<close>
+  "The Isabelle Cookbook" section 2.3.\<close>
 
 text\<open>An omnipresent data-structure in the Isabelle SML sources are tables
-implemented in @{file "$ISABELLE_HOME/src/Pure/General/table.ML"}. These 
-generic tables are presented in an efficient purely functional implementation using
-balanced 2-3 trees. Key operations are:\<close>
+  implemented in @{file "$ISABELLE_HOME/src/Pure/General/table.ML"}. These 
+  generic tables are presented in an efficient purely functional implementation using
+  balanced 2-3 trees. Key operations are:\<close>
 ML\<open>
 signature TABLE_reduced =
 sig
@@ -246,45 +242,45 @@ chapter*[t2::technical] \<open>  Prover Architecture \<close>
 section*[t21::technical] \<open>  The Nano-Kernel: Contexts,  (Theory)-Contexts, (Proof)-Contexts \<close>
 
 text\<open> What I call the 'Nano-Kernel' in Isabelle can also be seen as an acyclic theory graph.
-The meat of it can be found in the file @{file "$ISABELLE_HOME/src/Pure/context.ML"}. 
-My notion is a bit criticisable since this component, which provides the type of @{ML_type theory}
-and @{ML_type Proof.context},  is not that Nano after all.
-However, these type are pretty empty place-holders at that level and the content of
-@{file  "$ISABELLE_HOME/src/Pure/theory.ML"} is registered much later.
-The sources themselves mention it as "Fundamental Structure".
-In principle, theories and proof contexts could be REGISTERED as user data inside contexts.
-The chosen specialization is therefore an acceptable meddling of the abstraction "Nano-Kernel"
-and its application context: Isabelle.
-
-Makarius himself says about this structure:
-
-"Generic theory contexts with unique identity, arbitrarily typed data,
-monotonic development graph and history support.  Generic proof
-contexts with arbitrarily typed data."
-
-In my words: a context is essentially a container with
-\<^item> an id
-\<^item> a list of parents (so: the graph structure)
-\<^item> a time stamp and
-\<^item> a sub-context relation (which uses a combination of the id and the time-stamp to
-  establish this relation very fast whenever needed; it plays a crucial role for the
-  context transfer in the kernel.
-
-
-A context comes in form of three 'flavours':
-\<^item> theories : @{ML_type theory}'s, containing a syntax and axioms, but also
-             user-defined data and configuration information.
-\<^item> Proof-Contexts:  @{ML_type Proof.context} 
-             containing theories but also additional information if Isar goes into prove-mode.
-             In general a richer structure than theories coping also with fixes, facts, goals,
-             in order to support the structured Isar proof-style.
-\<^item> Generic:  @{ML_type Context.generic }, i.e. the sum of both.
-
-All context have to be seen as mutable; so there are usually transformations defined on them
-which are possible as long as a particular protocol (\<^verbatim>\<open>begin_thy\<close> - \<^verbatim>\<open>end_thy\<close> etc) are respected.
-
-Contexts come with type user-defined data which is mutable through the entire lifetime of
-a context.
+  The meat of it can be found in the file @{file "$ISABELLE_HOME/src/Pure/context.ML"}. 
+  My notion is a bit criticisable since this component, which provides the type of @{ML_type theory}
+  and @{ML_type Proof.context},  is not that Nano after all.
+  However, these type are pretty empty place-holders at that level and the content of
+  @{file  "$ISABELLE_HOME/src/Pure/theory.ML"} is registered much later.
+  The sources themselves mention it as "Fundamental Structure".
+  In principle, theories and proof contexts could be REGISTERED as user data inside contexts.
+  The chosen specialization is therefore an acceptable meddling of the abstraction "Nano-Kernel"
+  and its application context: Isabelle.
+  
+  Makarius himself says about this structure:
+  
+  "Generic theory contexts with unique identity, arbitrarily typed data,
+  monotonic development graph and history support.  Generic proof
+  contexts with arbitrarily typed data."
+  
+  In my words: a context is essentially a container with
+  \<^item> an id
+  \<^item> a list of parents (so: the graph structure)
+  \<^item> a time stamp and
+  \<^item> a sub-context relation (which uses a combination of the id and the time-stamp to
+    establish this relation very fast whenever needed; it plays a crucial role for the
+    context transfer in the kernel.
+  
+  
+  A context comes in form of three 'flavours':
+  \<^item> theories : @{ML_type theory}'s, containing a syntax and axioms, but also
+               user-defined data and configuration information.
+  \<^item> Proof-Contexts:  @{ML_type Proof.context} 
+               containing theories but also additional information if Isar goes into prove-mode.
+               In general a richer structure than theories coping also with fixes, facts, goals,
+               in order to support the structured Isar proof-style.
+  \<^item> Generic:  @{ML_type Context.generic }, i.e. the sum of both.
+  
+  All context have to be seen as mutable; so there are usually transformations defined on them
+  which are possible as long as a particular protocol (\<^verbatim>\<open>begin_thy\<close> - \<^verbatim>\<open>end_thy\<close> etc) are respected.
+  
+  Contexts come with type user-defined data which is mutable through the entire lifetime of
+  a context.
 \<close>  
 
 subsection*[t212::technical]\<open> Mechanism 1 : Core Interface. \<close>
@@ -311,13 +307,15 @@ ML\<open>
 
 
 subsection*[t213::example]\<open>Mechanism 2 : Extending the Global Context $\theta$ by User Data \<close>
+
 text\<open>A central mechanism for constructing user-defined data is by the \<^verbatim>\<open>Generic_Data\<close> SML functor.
-A plugin needing some data \<^verbatim>\<open>T\<close> and providing it with implementations for an 
-\<^verbatim>\<open>empty\<close>, and operations  \<^verbatim>\<open>merge\<close> and \<^verbatim>\<open>extend\<close>, can construct a lense with operations
-\<^verbatim>\<open>get\<close> and \<^verbatim>\<open>put\<close> that attach this data into the generic system context. Rather than using
-unsynchronized SML mutable variables, this is the mechanism to introduce component local
-data in Isabelle, which allows to manage this data for the necessary backtrack- and synchronization
-features in the pervasively parallel evaluation framework that Isabelle as a system represents.\<close>
+  A plugin needing some data \<^verbatim>\<open>T\<close> and providing it with implementations for an 
+  \<^verbatim>\<open>empty\<close>, and operations  \<^verbatim>\<open>merge\<close> and \<^verbatim>\<open>extend\<close>, can construct a lense with operations
+  \<^verbatim>\<open>get\<close> and \<^verbatim>\<open>put\<close> that attach this data into the generic system context. Rather than using
+  unsynchronized SML mutable variables, this is the mechanism to introduce component local
+  data in Isabelle, which allows to manage this data for the necessary backtrack- and synchronization
+  features in the pervasively parallel evaluation framework that Isabelle as a system represents.\<close>
+
 ML \<open>
 datatype X = mt
 val init = mt;
@@ -354,7 +352,7 @@ text\<open>The classical LCF-style \<^emph>\<open>kernel\<close> is about
 
 subsection*[termstypes::technical]\<open> Terms and Types \<close>
 text \<open>A basic data-structure of the kernel is @{file "$ISABELLE_HOME/src/Pure/term.ML"} \<close>  
-ML\<open> open Term;
+ML\<open> (* open Term; *)
 signature TERM' = sig
   (* ... *)
   type indexname = string * int
@@ -406,34 +404,33 @@ text\<open>Note that the SML interpreter is configured that he will actually pri
      pretty much like a string. This can be confusing at times.\<close>
 
 text\<open>Note, furthermore, that there is a programming API for the HOL-instance of Isabelle:
-it is contained in @{file  "$ISABELLE_HOME/src/HOL/Tools/hologic.ML"}. It offers for many
-operators of the HOL logic specific constructors and destructors:
-\<close>
+  it is contained in @{file  "$ISABELLE_HOME/src/HOL/Tools/hologic.ML"}. It offers for many
+  operators of the HOL logic specific constructors and destructors:\<close>
 
 ML\<open>
-HOLogic.boolT         : typ;
-HOLogic.mk_Trueprop   : term -> term; (* the embedder of bool to prop fundamenyal for HOL *)
-HOLogic.dest_Trueprop : term -> term; 
-HOLogic.Trueprop_conv : conv -> conv;
-HOLogic.mk_setT       : typ -> typ;   (* ML level type constructor set *)
-HOLogic.dest_setT     : typ -> typ;
-HOLogic.Collect_const : typ -> term;
-HOLogic.mk_Collect    : string * typ * term -> term;
-HOLogic.mk_mem        : term * term -> term;
-HOLogic.dest_mem      : term -> term * term;
-HOLogic.mk_set        : typ -> term list -> term;
-HOLogic.conj_intr     : Proof.context -> thm -> thm -> thm; (* some HOL-level derived-inferences *)
-HOLogic.conj_elim     : Proof.context -> thm -> thm * thm;
-HOLogic.conj_elims    : Proof.context -> thm -> thm list;
-HOLogic.conj          : term;         (* some ML level logical constructors *)
-HOLogic.disj          : term;
-HOLogic.imp           : term;
-HOLogic.Not           : term;
-HOLogic.mk_not        : term -> term;
-HOLogic.mk_conj       : term * term -> term;
-HOLogic.dest_conj     : term -> term list;
-HOLogic.conjuncts     : term -> term list;
-(* ... *)
+   HOLogic.boolT         : typ;
+   HOLogic.mk_Trueprop   : term -> term; (* the embedder of bool to prop fundamenyal for HOL *)
+   HOLogic.dest_Trueprop : term -> term; 
+   HOLogic.Trueprop_conv : conv -> conv;
+   HOLogic.mk_setT       : typ -> typ;   (* ML level type constructor set *)
+   HOLogic.dest_setT     : typ -> typ;
+   HOLogic.Collect_const : typ -> term;
+   HOLogic.mk_Collect    : string * typ * term -> term;
+   HOLogic.mk_mem        : term * term -> term;
+   HOLogic.dest_mem      : term -> term * term;
+   HOLogic.mk_set        : typ -> term list -> term;
+   HOLogic.conj_intr     : Proof.context -> thm -> thm -> thm; (* some HOL-level derived-inferences *)
+   HOLogic.conj_elim     : Proof.context -> thm -> thm * thm;
+   HOLogic.conj_elims    : Proof.context -> thm -> thm list;
+   HOLogic.conj          : term;         (* some ML level logical constructors *)
+   HOLogic.disj          : term;
+   HOLogic.imp           : term;
+   HOLogic.Not           : term;
+   HOLogic.mk_not        : term -> term;
+   HOLogic.mk_conj       : term * term -> term;
+   HOLogic.dest_conj     : term -> term list;
+   HOLogic.conjuncts     : term -> term list;
+   (* ... *)
 \<close>
 
 
@@ -447,27 +444,27 @@ text\<open> there is a joker type that can be added as place-holder during term 
 ML\<open>  Term.dummyT : typ \<close>
 
 ML\<open>
-Sign.typ_instance: theory -> typ * typ -> bool;
-Sign.typ_match: theory -> typ * typ -> Type.tyenv -> Type.tyenv;
-Sign.typ_unify: theory -> typ * typ -> Type.tyenv * int -> Type.tyenv * int;
-Sign.const_type: theory -> string -> typ option;
-Sign.certify_term: theory -> term -> term * typ * int;   (* core routine for CERTIFICATION of types*)
-Sign.cert_term: theory -> term -> term;                  (* short-cut for the latter *)
-Sign.tsig_of: theory -> Type.tsig                        (* projects the type signature *)
+   Sign.typ_instance: theory -> typ * typ -> bool;
+   Sign.typ_match: theory -> typ * typ -> Type.tyenv -> Type.tyenv;
+   Sign.typ_unify: theory -> typ * typ -> Type.tyenv * int -> Type.tyenv * int;
+   Sign.const_type: theory -> string -> typ option;
+   Sign.certify_term: theory -> term -> term * typ * int;   (* core routine for CERTIFICATION of types*)
+   Sign.cert_term: theory -> term -> term;                  (* short-cut for the latter *)
+   Sign.tsig_of: theory -> Type.tsig                        (* projects the type signature *)
 \<close>
 text\<open> 
-@{ML "Sign.typ_match"} etc. is actually an abstract wrapper on the structure 
-@{ML_structure "Type"} 
-which contains the heart of the type inference. 
-It also contains the type substitution type  @{ML_type "Type.tyenv"} which is
-is actually a type synonym for @{ML_type "(sort * typ) Vartab.table"} 
-which in itself is a synonym for @{ML_type "'a Symtab.table"}, so 
-possesses the usual @{ML "Symtab.empty"} and  @{ML "Symtab.dest"} operations. \<close>  
+  @{ML "Sign.typ_match"} etc. is actually an abstract wrapper on the structure 
+  @{ML_structure "Type"} 
+  which contains the heart of the type inference. 
+  It also contains the type substitution type  @{ML_type "Type.tyenv"} which is
+  is actually a type synonym for @{ML_type "(sort * typ) Vartab.table"} 
+  which in itself is a synonym for @{ML_type "'a Symtab.table"}, so 
+  possesses the usual @{ML "Symtab.empty"} and  @{ML "Symtab.dest"} operations. \<close>  
 
 text\<open>Note that @{emph \<open>polymorphic variables\<close>} are treated like constant symbols 
-in the type inference; thus, the following test, that one type is an instance of the
-other, yields false:
-\<close>
+  in the type inference; thus, the following test, that one type is an instance of the
+  other, yields false:\<close>
+
 ML\<open>
 val ty = @{typ "'a option"};
 val ty' = @{typ "int option"};
@@ -477,13 +474,14 @@ val Type("List.list",[S]) = @{typ "('a) list"}; (* decomposition example *)
 val false = Sign.typ_instance @{theory}(ty', ty);
 \<close>
 text\<open>In order to make the type inference work, one has to consider @{emph \<open>schematic\<close>} 
-type variables, which are more and more hidden from the Isar interface. Consequently,
-the typ antiquotation above will not work for schematic type variables and we have
-to construct them by hand on the SML level: \<close>
-ML\<open> 
-val t_schematic = Type("List.list",[TVar(("'a",0),@{sort "HOL.type"})]);
-\<close>
+  type variables, which are more and more hidden from the Isar interface. Consequently,
+  the typ antiquotation above will not work for schematic type variables and we have
+  to construct them by hand on the SML level: \<close>
+
+ML\<open> val t_schematic = Type("List.list",[TVar(("'a",0),@{sort "HOL.type"})]); \<close>
+
 text\<open> MIND THE "'" !!!\<close>
+
 text \<open>On this basis, the following @{ML_type "Type.tyenv"} is constructed: \<close>
 ML\<open>
 val tyenv = Sign.typ_match ( @{theory}) 
@@ -493,9 +491,9 @@ val  [(("'a", 0), (["HOL.type"], @{typ "int"}))] = Vartab.dest tyenv;
 \<close>
 
 text\<open> Type generalization --- the conversion between free type variables and schematic 
-type variables ---  is apparently no longer part of the standard API (there is a slightly 
-more general replacement in @{ML "Term_Subst.generalizeT_same"}, however). Here is a way to
-overcome this by a self-baked generalization function:\<close>  
+  type variables ---  is apparently no longer part of the standard API (there is a slightly 
+  more general replacement in @{ML "Term_Subst.generalizeT_same"}, however). Here is a way to
+  overcome this by a self-baked generalization function:\<close>  
 
 ML\<open>
 val generalize_typ = Term.map_type_tfree (fn (str,sort)=> Term.TVar((str,0),sort));
@@ -503,16 +501,14 @@ val generalize_term = Term.map_types generalize_typ;
 val true = Sign.typ_instance @{theory} (ty', generalize_typ ty)
 \<close>
 text\<open>... or more general variants thereof that are parameterized by the indexes for schematic
-type variables instead of assuming just @{ML "0"}. \<close>
+  type variables instead of assuming just @{ML "0"}. \<close>
 
 text*[exo4::example]\<open> Example:\<close> 
 ML\<open>val t = generalize_term @{term "[]"}\<close>
 
-text
-\<open>Now we turn to the crucial issue of type-instantiation and with a given type environment
-@{ML "tyenv"}. For this purpose, one has to switch to the low-level interface 
-@{ML_structure "Term_Subst"}. 
-\<close>
+text\<open>Now we turn to the crucial issue of type-instantiation and with a given type environment
+  @{ML "tyenv"}. For this purpose, one has to switch to the low-level interface 
+  @{ML_structure "Term_Subst"}. \<close>
 
 ML\<open>
 Term_Subst.map_types_same : (typ -> typ) -> term -> term;
@@ -529,7 +525,7 @@ Term_Subst.generalize: string list * string list -> int -> term -> term
 \<close>
 
 text \<open>Apparently, a bizarre conversion between the old-style interface and 
-the new-style @{ML "tyenv"} is necessary. See the following example.\<close>
+  the new-style @{ML "tyenv"} is necessary. See the following example.\<close>
 ML\<open>
 val S = Vartab.dest tyenv;
 val S' = (map (fn (s,(t,u)) => ((s,t),u)) S) : ((indexname * sort) * typ) list;
@@ -545,23 +541,18 @@ val t'' = Term.map_types (Term_Subst.instantiateT S') (t)
 \<close>
 
 text\<open>A more abstract env for variable management in tactic proofs. A bit difficult to use
-outside the very closed-up tracks of conventional use...\<close>
+  outside the very closed-up tracks of conventional use...\<close>
 
-ML\<open>
-Consts.the_const; (* T is a kind of signature ... *)
-Variable.import_terms;
-Vartab.update;
-\<close>
+ML\<open> Consts.the_const; (* T is a kind of signature ... *)
+    Variable.import_terms;
+    Vartab.update;\<close>
 
 subsection*[t232::technical]\<open> Type-Inference (= inferring consistent type information if possible) \<close>
 
 text\<open> Type inference eliminates also joker-types such as @{ML dummyT} and produces
        instances for schematic type variables where necessary. In the case of success,
        it produces a certifiable term. \<close>  
-ML\<open>  
-Type_Infer_Context.infer_types: Proof.context -> term list -> term list  
-\<close>
-
+ML\<open>  Type_Infer_Context.infer_types: Proof.context -> term list -> term list \<close>
 
   
 subsection*[t233::technical]\<open> Theories and the Signature API\<close>  
@@ -652,12 +643,12 @@ text\<open>Note that the transfer rule:
  \Gamma \vdash_{\theta'} \phi  \qquad \qquad
 \end{prooftree}
 \]
-which is a consequence of explicit theories  characteristic for Isabelle's LCF-kernel design
-and a remarkable difference to its sisters HOL-Light and HOL4; instead of transfer, these systems
-reconstruct proofs in an enlarged global context instead of taking the result and converting it.\<close>
+  which is a consequence of explicit theories  characteristic for Isabelle's LCF-kernel design
+  and a remarkable difference to its sisters HOL-Light and HOL4; instead of transfer, these systems
+  reconstruct proofs in an enlarged global context instead of taking the result and converting it.\<close>
 
 text\<open>Besides the meta-logical (Pure) implication $\_\Longrightarrow \_$, the Kernel axiomatizes
-also a Pure-Equality $\_ \equiv \_ $ used for definitions of constant symbols: \<close>
+  also a Pure-Equality $\_ \equiv \_ $ used for definitions of constant symbols: \<close>
 ML\<open>
   Thm.reflexive: cterm -> thm;
   Thm.symmetric: thm -> thm;
@@ -691,10 +682,9 @@ ML\<open>
 subsection*[t235::technical]\<open> Theories \<close>
 
 text \<open> This structure yields the datatype \verb*thy* which becomes the content of 
-\verb*Context.theory*. In a way, the LCF-Kernel registers itself into the Nano-Kernel,
-which inspired me (bu) to this naming. 
+  \verb*Context.theory*. In a way, the LCF-Kernel registers itself into the Nano-Kernel,
+  which inspired me (bu) to this naming. \<close>
 
-\<close>
 ML\<open>
 
 (* intern Theory.Thy; 
@@ -721,29 +711,26 @@ Theory.defs_of: theory -> Defs.T;
 Theory.at_begin: (theory -> theory option) -> theory -> theory;
 Theory.at_end: (theory -> theory option) -> theory -> theory;
 Theory.begin_theory: string * Position.T -> theory list -> theory;
-Theory.end_theory: theory -> theory;
-
-\<close>
+Theory.end_theory: theory -> theory;\<close>
 
 
 section*[t24::technical]\<open>Backward Proofs: Tactics, Tacticals and Goal-States\<close>
 
 text\<open>At this point, we leave the Pure-Kernel and start to describe the first layer on top
-of it, involving support for specific styles of reasoning and automation of reasoning.\<close>
+  of it, involving support for specific styles of reasoning and automation of reasoning.\<close>
 
 text\<open> \<^verbatim>\<open>tactic\<close>'s are in principle \<^emph>\<open>relations\<close> on theorems @{ML_type "thm"}; this gives a natural way 
-to represent the fact that HO-Unification (and therefore the mechanism of rule-instantiation) 
-are non-deterministic in principle. Heuristics may choose particular preferences between 
-the theorems in the range of this relation, but the Isabelle Design accepts this fundamental 
-fact reflected at this point in the prover architecture. 
-This potentially infinite relation is implemented by a function of theorems to lazy lists 
-over theorems, which gives both sufficient structure for heuristic
-considerations as well as a nice algebra, called  \<^verbatim>\<open>TACTICAL\<close>'s, providing a bottom element
-@{ML "no_tac"} (the function that always fails), the top-element @{ML "all_tac"}
- (the function that never fails), sequential composition @{ML "op THEN"}, (serialized) 
-non-deterministic composition @{ML "op ORELSE"}, conditionals, repetitions over lists, etc.
-The following is an excerpt of @{file "~~/src/Pure/tactical.ML"}:
-\<close>
+  to represent the fact that HO-Unification (and therefore the mechanism of rule-instantiation) 
+  are non-deterministic in principle. Heuristics may choose particular preferences between 
+  the theorems in the range of this relation, but the Isabelle Design accepts this fundamental 
+  fact reflected at this point in the prover architecture. 
+  This potentially infinite relation is implemented by a function of theorems to lazy lists 
+  over theorems, which gives both sufficient structure for heuristic
+  considerations as well as a nice algebra, called  \<^verbatim>\<open>TACTICAL\<close>'s, providing a bottom element
+  @{ML "no_tac"} (the function that always fails), the top-element @{ML "all_tac"}
+   (the function that never fails), sequential composition @{ML "op THEN"}, (serialized) 
+  non-deterministic composition @{ML "op ORELSE"}, conditionals, repetitions over lists, etc.
+  The following is an excerpt of @{file "~~/src/Pure/tactical.ML"}:\<close>
 
 ML\<open>
 signature TACTICAL =
@@ -768,21 +755,20 @@ end
 \<close>
 
 text\<open>The next layer in the architecture describes @{ML_type \<open>tactic\<close>}'s, i.e. basic operations on 
-theorems  in a backward reasoning style (bottom up development of proof-trees). An initial goal-state 
-for some property @{term A} --- the \<^emph>\<open>goal\<close> --- is constructed via the kernel 
-@{ML "Thm.trivial"}-operation into  @{term "A \<Longrightarrow> A"}, and tactics either refine the premises 
---- the \<^emph>\<open>subgoals\<close> the of this meta-implication --- 
-producing more and more of them or eliminate them in subsequent goal-states. Subgoals of the form  
-@{term "B\<^sub>1 \<Longrightarrow> B\<^sub>2 \<Longrightarrow> A \<Longrightarrow> B\<^sub>3 \<Longrightarrow> B\<^sub>4 \<Longrightarrow> A"} can be eliminated via 
-the @{ML Tactic.assume_tac} - tactic, 
-and a subgoal @{term C\<^sub>m} can be refined via the theorem
-@{term "E\<^sub>1 \<Longrightarrow> E\<^sub>2 \<Longrightarrow> E\<^sub>3 \<Longrightarrow> C\<^sub>m"} the @{ML Tactic.resolve_tac} - tactic to new subgoals
-@{term "E\<^sub>1"},@{term "E\<^sub>2"}, @{term "E\<^sub>3"}. In case that a theorem used for resolution
-has no premise @{term "E\<^sub>i"}, the subgoal  @{term C\<^sub>m} is also eliminated ("closed").
-
-The following abstract of the most commonly used @{ML_type \<open>tactic\<close>}'s drawn from
-@{file "~~/src/Pure/tactic.ML"} looks as follows:
-\<close>
+  theorems  in a backward reasoning style (bottom up development of proof-trees). An initial goal-state 
+  for some property @{term A} --- the \<^emph>\<open>goal\<close> --- is constructed via the kernel 
+  @{ML "Thm.trivial"}-operation into  @{term "A \<Longrightarrow> A"}, and tactics either refine the premises 
+  --- the \<^emph>\<open>subgoals\<close> the of this meta-implication --- 
+  producing more and more of them or eliminate them in subsequent goal-states. Subgoals of the form  
+  @{term "B\<^sub>1 \<Longrightarrow> B\<^sub>2 \<Longrightarrow> A \<Longrightarrow> B\<^sub>3 \<Longrightarrow> B\<^sub>4 \<Longrightarrow> A"} can be eliminated via 
+  the @{ML Tactic.assume_tac} - tactic, 
+  and a subgoal @{term C\<^sub>m} can be refined via the theorem
+  @{term "E\<^sub>1 \<Longrightarrow> E\<^sub>2 \<Longrightarrow> E\<^sub>3 \<Longrightarrow> C\<^sub>m"} the @{ML Tactic.resolve_tac} - tactic to new subgoals
+  @{term "E\<^sub>1"},@{term "E\<^sub>2"}, @{term "E\<^sub>3"}. In case that a theorem used for resolution
+  has no premise @{term "E\<^sub>i"}, the subgoal  @{term C\<^sub>m} is also eliminated ("closed").
+  
+  The following abstract of the most commonly used @{ML_type \<open>tactic\<close>}'s drawn from
+  @{file "~~/src/Pure/tactic.ML"} looks as follows:\<close>
 
 ML\<open>
   (* ... *)
@@ -798,8 +784,8 @@ ML\<open>
   (* ... *)
 \<close>
 text\<open>Note that "applying a rule" is a fairly complex operation in the Extended Isabelle Kernel,
-i.e. the tactic layer. It involves at least four phases, interfacing a theorem
-coming from the global context $\theta$ (=theory), be it axiom or derived, into a given goal-state.
+  i.e. the tactic layer. It involves at least four phases, interfacing a theorem 
+  coming from the global context $\theta$ (=theory), be it axiom or derived, into a given goal-state.
 \<^item> \<^emph>\<open>generalization\<close>. All free variables in the theorem were replaced by schematic variables.
   For example, @{term "x + y = y + x"} is converted into 
   @{emph \<open>?x + ?y = ?y + ?x\<close> }. 
@@ -833,16 +819,16 @@ coming from the global context $\theta$ (=theory), be it axiom or derived, into 
 \<close>
 
 text\<open>In a way, the two lifting processes represent an implementation of the conversion between
-Gentzen Natural Deduction (to which Isabelle/Pure is geared) reasoning and 
-Gentzen Sequent Deduction.\<close>
+  Gentzen Natural Deduction (to which Isabelle/Pure is geared) reasoning and 
+  Gentzen Sequent Deduction.\<close>
 
 
 section*[goalp::technical]\<open>The classical goal package\<close>
 text\<open>The main mechanism in Isabelle as an LCF-style system is to produce @{ML_type thm}'s 
-in backward-style via tactics as described in @{technical "t24"}. Given a context
---- be it global as @{ML_type theory} or be it inside a proof-context as @{ML_type Proof.context},
-user-programmed verification of (type-checked) terms or just strings can be done via the operations:
-\<close>
+  in backward-style via tactics as described in @{technical "t24"}. Given a context
+  --- be it global as @{ML_type theory} or be it inside a proof-context as @{ML_type Proof.context},
+  user-programmed verification of (type-checked) terms or just strings can be done via the 
+  operations:\<close>
 
 
 ML\<open>
@@ -853,7 +839,7 @@ Goal.prove_global :  theory -> string list -> term list -> term ->
 (* ... and many more variants. *)
 \<close>
 
-subsection*[ex211::example]\<open>Proof example\<close>
+subsection*[ex211::example]\<open>Proof Example\<close>
 
 text\<open>The proof:\<close>
 
@@ -870,16 +856,8 @@ val thm1 = Goal.prove_global @{theory}                         (* global context
                              []                                (* name ? *)
                              []                                (* local assumption context *)
                              (tt)                              (* parsed goal *)
-                             (fn _ => simp_tac  @{context} 1)  (* proof tactic *)
-\<close>               
+                             (fn _ => simp_tac  @{context} 1)  (* proof tactic *)\<close>               
 
-
-
-subsection*[exo44::example]\<open>Example\<close>
-
-ML\<open>
-Goal.prove_global @{theory} ["2::int + 3 = 5"] 
-\<close>
 
 section\<open>The Isar Engine\<close>
 
@@ -888,20 +866,19 @@ internal @{ ML_type state} with the necessary infrastructure ---
 i.e. the operations to pack and unpack theories and Proof.contexts  --- on it:
 \<close>
 ML\<open> 
- Toplevel.theory_toplevel: theory -> Toplevel.state;
- Toplevel.init_toplevel: unit -> Toplevel.state;
- Toplevel.is_toplevel: Toplevel.state -> bool;
- Toplevel.is_theory: Toplevel.state -> bool;
- Toplevel.is_proof: Toplevel.state -> bool;
- Toplevel.is_skipped_proof: Toplevel.state -> bool;
- Toplevel.level: Toplevel.state -> int;
- Toplevel.context_of: Toplevel.state -> Proof.context;
- Toplevel.generic_theory_of: Toplevel.state -> generic_theory;
- Toplevel.theory_of: Toplevel.state -> theory;
- Toplevel.proof_of: Toplevel.state -> Proof.state;
- Toplevel.presentation_context: Toplevel.state -> Proof.context;
-
-\<close>
+    Toplevel.theory_toplevel: theory -> Toplevel.state;
+    Toplevel.init_toplevel: unit -> Toplevel.state;
+    Toplevel.is_toplevel: Toplevel.state -> bool;
+    Toplevel.is_theory: Toplevel.state -> bool;
+    Toplevel.is_proof: Toplevel.state -> bool;
+    Toplevel.is_skipped_proof: Toplevel.state -> bool;
+    Toplevel.level: Toplevel.state -> int;
+    Toplevel.context_of: Toplevel.state -> Proof.context;
+    Toplevel.generic_theory_of: Toplevel.state -> generic_theory;
+    Toplevel.theory_of: Toplevel.state -> theory;
+    Toplevel.proof_of: Toplevel.state -> Proof.state;
+    Toplevel.presentation_context: Toplevel.state -> Proof.context;
+    (* ... *) \<close>
 
 text\<open> The extensibility of Isabelle as a system framework depends on a number of tables,
   into which various concepts commands, ML-antiquotations, text-antiquotations, cartouches, ...
@@ -914,8 +891,7 @@ text\<open> The extensibility of Isabelle as a system framework depends on a num
   creates an implicit  @{ML Theory.setup}  with an entry for a call-back function, which happens
   to be a parser that must have as side-effect a Toplevel-transition-transition. 
   Registers @{ML_type "Toplevel.transition -> Toplevel.transition"} parsers to the 
-  Isar interpreter.
-\<close>
+  Isar interpreter.\<close>
 
 
 ML\<open> Outer_Syntax.command : Outer_Syntax.command_keyword -> string -> 
@@ -940,31 +916,62 @@ ML\<open> Thy_Header.get_keywords @{theory};(* this looks to be really theory gl
 
 subsection*[transmgt::technical] \<open>Transaction Management in the Isar-Engine : The Toplevel \<close>
   
+ML\<open>Toplevel.exit: Toplevel.transition -> Toplevel.transition;
+  Toplevel.keep: (Toplevel.state -> unit) -> Toplevel.transition -> Toplevel.transition;
+  Toplevel.keep': (bool -> Toplevel.state -> unit) -> Toplevel.transition -> Toplevel.transition;
+  Toplevel.ignored: Position.T -> Toplevel.transition;
+  Toplevel.generic_theory: (generic_theory -> generic_theory) -> Toplevel.transition -> Toplevel.transition;
+  Toplevel.theory': (bool -> theory -> theory) -> Toplevel.transition -> Toplevel.transition;
+  Toplevel.theory: (theory -> theory) -> Toplevel.transition -> Toplevel.transition;
+  
+  Toplevel.present_local_theory:
+  (xstring * Position.T) option ->
+       (Toplevel.state -> unit) -> Toplevel.transition -> Toplevel.transition;
+  (* where text treatment and antiquotation parsing happens *)
+  
+  
+  (*fun document_command markdown (loc, txt) =
+    Toplevel.keep (fn state =>
+      (case loc of
+        NONE => ignore (output_text state markdown txt)
+      | SOME (_, pos) =>
+          error ("Illegal target specification -- not a theory context" ^ Position.here pos))) o
+    Toplevel.present_local_theory loc (fn state => ignore (output_text state markdown txt)); *)
+  
+  (* Isar Toplevel Steuerung *)
+  Toplevel.keep :  (Toplevel.state -> unit) -> Toplevel.transition -> Toplevel.transition;
+      (* val keep' = add_trans o Keep;
+         fun keep f = add_trans (Keep (fn _ => f));
+       *)
+  
+  Toplevel.present_local_theory : (xstring * Position.T) option -> (Toplevel.state -> unit) ->
+      Toplevel.transition -> Toplevel.transition;
+      (* fun present_local_theory target = present_transaction (fn int =>
+             (fn Theory (gthy, _) =>
+                     let val (finish, lthy) = Named_Target.switch target gthy;
+                     in Theory (finish lthy, SOME lthy) end
+             | _ => raise UNDEF));
+  
+         fun present_transaction f g = add_trans (Transaction (f, g));
+         fun transaction f = present_transaction f (K ());
+      *)
+  
+  Toplevel.theory : (theory -> theory) -> Toplevel.transition -> Toplevel.transition; 
+     (* fun theory' f = transaction (fn int =>
+                  (fn Theory (Context.Theory thy, _) =>
+                        let val thy' = thy
+                                       |> Sign.new_group
+                                       |> f int
+                                       |> Sign.reset_group;
+                        in Theory (Context.Theory thy', NONE) end
+                  | _ => raise UNDEF));
+  
+        fun theory f = theory' (K f); *)\<close>  
+  
+  
 ML\<open>
 
-Toplevel.exit: Toplevel.transition -> Toplevel.transition;
-Toplevel.keep: (Toplevel.state -> unit) -> Toplevel.transition -> Toplevel.transition;
-Toplevel.keep': (bool -> Toplevel.state -> unit) -> Toplevel.transition -> Toplevel.transition;
-Toplevel.ignored: Position.T -> Toplevel.transition;
-Toplevel.generic_theory: (generic_theory -> generic_theory) -> Toplevel.transition -> Toplevel.transition;
-Toplevel.theory': (bool -> theory -> theory) -> Toplevel.transition -> Toplevel.transition;
-Toplevel.theory: (theory -> theory) -> Toplevel.transition -> Toplevel.transition;
-
-Toplevel.present_local_theory:
-(xstring * Position.T) option ->
-     (Toplevel.state -> unit) -> Toplevel.transition -> Toplevel.transition;
-(* where text treatment and antiquotation parsing happens *)
-
-
-(*fun document_command markdown (loc, txt) =
-  Toplevel.keep (fn state =>
-    (case loc of
-      NONE => ignore (output_text state markdown txt)
-    | SOME (_, pos) =>
-        error ("Illegal target specification -- not a theory context" ^ Position.here pos))) o
-  Toplevel.present_local_theory loc (fn state => ignore (output_text state markdown txt)); *)
-
-(* Isar Toplevel Steuerung *)
+(* Isar Toplevel Control *)
 Toplevel.keep :  (Toplevel.state -> unit) -> Toplevel.transition -> Toplevel.transition;
     (* val keep' = add_trans o Keep;
        fun keep f = add_trans (Keep (fn _ => f));
@@ -993,62 +1000,23 @@ Toplevel.theory : (theory -> theory) -> Toplevel.transition -> Toplevel.transiti
                 | _ => raise UNDEF));
 
       fun theory f = theory' (K f); *)
-
-\<close>  
-  
-  
-ML\<open>
-
-
-(* Isar Toplevel Steuerung *)
-Toplevel.keep :  (Toplevel.state -> unit) -> Toplevel.transition -> Toplevel.transition;
-    (* val keep' = add_trans o Keep;
-       fun keep f = add_trans (Keep (fn _ => f));
-     *)
-
-Toplevel.present_local_theory : (xstring * Position.T) option -> (Toplevel.state -> unit) ->
-    Toplevel.transition -> Toplevel.transition;
-    (* fun present_local_theory target = present_transaction (fn int =>
-           (fn Theory (gthy, _) =>
-                   let val (finish, lthy) = Named_Target.switch target gthy;
-                   in Theory (finish lthy, SOME lthy) end
-           | _ => raise UNDEF));
-
-       fun present_transaction f g = add_trans (Transaction (f, g));
-       fun transaction f = present_transaction f (K ());
-    *)
-
-Toplevel.theory : (theory -> theory) -> Toplevel.transition -> Toplevel.transition; 
-   (* fun theory' f = transaction (fn int =>
-                (fn Theory (Context.Theory thy, _) =>
-                      let val thy' = thy
-                                     |> Sign.new_group
-                                     |> f int
-                                     |> Sign.reset_group;
-                      in Theory (Context.Theory thy', NONE) end
-                | _ => raise UNDEF));
-
-      fun theory f = theory' (K f); *)
-
-
 \<close>
   
   
 subsection*[conf::technical]\<open> Configuration flags of fixed type in the Isar-engine. \<close>
 text\<open>The toplevel also provides an infrastructure for managing configuration options 
-for system components. Based on a sum-type @{ML_type Config.value } 
-with the alternatives \<^verbatim>\<open> Bool of bool | Int of int | Real of real | String of string\<close>
-and building the parametric configuration types @{ML_type "'a Config.T" } and the
-instance  \<^verbatim>\<open>type raw = value T\<close>, for all registered configurations the protocol:
-\<close>
+  for system components. Based on a sum-type @{ML_type Config.value } 
+  with the alternatives \<^verbatim>\<open> Bool of bool | Int of int | Real of real | String of string\<close>
+  and building the parametric configuration types @{ML_type "'a Config.T" } and the
+  instance  \<^verbatim>\<open>type raw = value T\<close>, for all registered configurations the protocol:\<close>
 ML\<open>
- Config.get: Proof.context -> 'a Config.T -> 'a;
- Config.map: 'a Config.T -> ('a -> 'a) -> Proof.context -> Proof.context;
- Config.put: 'a Config.T -> 'a -> Proof.context -> Proof.context;
- Config.get_global: theory -> 'a Config.T -> 'a;
- Config.map_global: 'a Config.T -> ('a -> 'a) -> theory -> theory;
- Config.put_global: 'a Config.T -> 'a -> theory -> theory;
-\<close>
+  Config.get: Proof.context -> 'a Config.T -> 'a;
+  Config.map: 'a Config.T -> ('a -> 'a) -> Proof.context -> Proof.context;
+  Config.put: 'a Config.T -> 'a -> Proof.context -> Proof.context;
+  Config.get_global: theory -> 'a Config.T -> 'a;
+  Config.map_global: 'a Config.T -> ('a -> 'a) -> theory -> theory;
+  Config.put_global: 'a Config.T -> 'a -> theory -> theory;\<close>
+
 text\<open>... etc. is defined.\<close>
 
 text\<open>Example registration of an config attribute XS232: \<close>
@@ -1056,8 +1024,7 @@ ML\<open>
 val (XS232, XS232_setup)
      = Attrib.config_bool \<^binding>\<open>XS232\<close> (K false);
 
-val _ = Theory.setup XS232_setup;
-\<close>
+val _ = Theory.setup XS232_setup;\<close>
 
 (* or: just command:
 
@@ -1068,79 +1035,77 @@ setup\<open>XS232_setup\<close>
 text\<open>Another mechanism are global synchronised variables:\<close>
 ML\<open> (* For example *)
            
-val C = Synchronized.var "Pretty.modes" "latEEex"; 
-(* Synchronized: a mechanism to bookkeep global
-   variables with synchronization mechanism included *)
-Synchronized.value C;
-\<close>  
+  val C = Synchronized.var "Pretty.modes" "latEEex"; 
+  (* Synchronized: a mechanism to bookkeep global
+     variables with synchronization mechanism included *)
+  Synchronized.value C;\<close>  
   
 chapter*[frontend::technical]\<open>Front-End \<close>  
 text\<open>In the following chapter, we turn to the right part of the system architecture 
-shown in @{docitem \<open>architecture\<close>}: 
-The PIDE ("Prover-IDE") layer @{cite "DBLP:conf/itp/Wenzel14"}
-consisting of a part written in SML and another in SCALA.
-Roughly speaking, PIDE implements "continuous build - continuous check" - functionality
-over a textual, albeit generic document model. It transforms user modifications
-of text elements in an instance of this model into increments (edits) and communicates
-them to the Isabelle system. The latter reacts by the creation of a multitude of light-weight
-reevaluation threads resulting in an asynchronous stream of markup that is used to annotate text
-elements. Such markup is used to highlight, e.g., variables
-or keywords with specific colors, to hyper-linking bound variables to their defining occurrences,
-or to annotate type-information to terms which becomes displayed by specific
-user-gestures on demand (hovering), etc. 
-Note that PIDE is not an editor, it is the framework that 
-coordinates these asynchronous information streams and optimizes it to a certain
-extent (outdated markup referring to modified text is dropped, and 
-corresponding re-calculations are oriented to the user focus, for example). 
-Four concrete editors --- also called PIDE applications --- have been implemented:
-\<^enum>an Eclipse plugin (developped by an Edinburg-group, based on an very old PIDE version),
-\<^enum>a Visual-Studio Code plugin (developed by Makarius Wenzel), 
- currently based on a fairly old PIDE version, 
-\<^enum>clide, a web-client supporting javascript and HTML5
- (developed by a group at University Bremen, based on a very old PIDE version), and 
-\<^enum>the most commonly used: the plugin in JEdit - Editor,
- (developed by Makarius Wenzel, current PIDE version.)
-\<close>
+  shown in @{docitem \<open>architecture\<close>}: 
+  The PIDE ("Prover-IDE") layer @{cite "DBLP:conf/itp/Wenzel14"}
+  consisting of a part written in SML and another in SCALA.
+  Roughly speaking, PIDE implements "continuous build - continuous check" - functionality
+  over a textual, albeit generic document model. It transforms user modifications
+  of text elements in an instance of this model into increments (edits) and communicates
+  them to the Isabelle system. The latter reacts by the creation of a multitude of light-weight
+  reevaluation threads resulting in an asynchronous stream of markup that is used to annotate text
+  elements. Such markup is used to highlight, e.g., variables
+  or keywords with specific colors, to hyper-linking bound variables to their defining occurrences,
+  or to annotate type-information to terms which becomes displayed by specific
+  user-gestures on demand (hovering), etc. 
+  Note that PIDE is not an editor, it is the framework that 
+  coordinates these asynchronous information streams and optimizes it to a certain
+  extent (outdated markup referring to modified text is dropped, and 
+  corresponding re-calculations are oriented to the user focus, for example). 
+  Four concrete editors --- also called PIDE applications --- have been implemented:
+\<^enum> an Eclipse plugin (developped by an Edinburg-group, based on an very old PIDE version),
+\<^enum> a Visual-Studio Code plugin (developed by Makarius Wenzel), 
+  currently based on a fairly old PIDE version, 
+\<^enum> clide, a web-client supporting javascript and HTML5
+  (developed by a group at University Bremen, based on a very old PIDE version), and 
+\<^enum> the most commonly used: the plugin in JEdit - Editor,
+  (developed by Makarius Wenzel, current PIDE version.)\<close>
 
-text\<open>The document model forsees a number of text files, which are organized in form of an acyclic graph. Such graphs can be 
-grouped into \<^emph>\<open>sessions\<close> and "frozen" to binaries in order to avoid long compilation 
-times. Text files have an abstract name serving as identity (the mapping to file-paths 
-in an underlying file-system is done in an own build management).
-The primary format of the text files is \<^verbatim>\<open>.thy\<close> (historically for: theory),
-secondary formats can be \<^verbatim>\<open>.sty\<close>,\<^verbatim>\<open>.tex\<close>, \<^verbatim>\<open>.png\<close>, \<^verbatim>\<open>.pdf\<close>, or other files processed 
-by Isabelle and listed in a configuration processed by the build system.
-\<close>
+text\<open>The document model forsees a number of text files, which are organized in form of an 
+  acyclic graph. Such graphs can be grouped into \<^emph>\<open>sessions\<close> and "frozen" to binaries in order 
+  to avoid long compilation times. Text files have an abstract name serving as identity (the 
+  mapping to file-paths in an underlying file-system is done in an own build management).
+  The primary format of the text files is \<^verbatim>\<open>.thy\<close> (historically for: theory),
+  secondary formats can be \<^verbatim>\<open>.sty\<close>,\<^verbatim>\<open>.tex\<close>, \<^verbatim>\<open>.png\<close>, \<^verbatim>\<open>.pdf\<close>, or other files processed 
+  by Isabelle and listed in a configuration processed by the build system.\<close>
+
 figure*[fig3::figure, relative_width="100",src="''figures/document-model''"]
         \<open>A Theory-Graph in the Document Model\<close>
-text\<open>A \<^verbatim>\<open>.thy\<close> file consists of a \<^emph>\<open>header\<close>, a \<^emph>\<open>context-definition\<close> and 
-a \<^emph>\<open>body\<close> consisting of a sequence of \<^emph>\<open>commands\<close>. Even the header consists of
-a sequence of commands used for introductory text elements not depending on any context
-information (so: practically excluding any form of text antiquotation (see above)).
-The context-definition contains an \<^emph>\<open>import\<close> and a \<^emph>\<open>keyword\<close> section;  
-for example:
-\begin{verbatim}
-theory Isa_DOF                (* Isabelle Document Ontology Framework *)
-  imports  Main  
-           RegExpInterface    (* Interface to functional regular automata for monitoring *)
-           Assert
-           
-  keywords "+=" ":=" "accepts" "rejects"
-\end{verbatim}
-where \<^verbatim>\<open>Isa_DOF\<close> is the abstract name of the text-file, \<^verbatim>\<open>Main\<close> etc. refer to imported
-text files (recall that the import relation must be acyclic). \<^emph>\<open>keyword\<close>s are used to separate 
-commands form each other;
-predefined commands allow for the dynamic creation of new commands similarly 
-to the definition of new functions in an interpreter shell (or: toplevel, see above.).
-A command starts with a pre-declared keyword and specific syntax of this command;
-the declaration of a keyword is only allowed in the same \<^verbatim>\<open>.thy\<close>-file where the
-the corresponding new command is defined. The semantics of the command is expressed
-in ML and consists of a @{ML_type "Toplevel.transition -> Toplevel.transition"}
-function. Thus, the Isar-toplevel supports the generic document model 
-and allows for user-programmed extensions.
-\<close>
+
+text\<open>A \<^verbatim>\<open>.thy\<close> file consists of a \<^emph>\<open>header\<close>, a \<^emph>\<open>context-definition\<close> and
+  a \<^emph>\<open>body\<close> consisting of a sequence of \<^emph>\<open>commands\<close>. Even the header consists of
+  a sequence of commands used for introductory text elements not depending on any context
+  information (so: practically excluding any form of text antiquotation (see above)).
+  The context-definition contains an \<^emph>\<open>import\<close> and a \<^emph>\<open>keyword\<close> section;  
+  for example:
+  \begin{verbatim}
+  theory Isa_DOF                (* Isabelle Document Ontology Framework *)
+    imports  Main  
+             RegExpInterface    (* Interface to functional regular automata for monitoring *)
+             Assert
+             
+    keywords "+=" ":=" "accepts" "rejects"
+  \end{verbatim}
+  where \<^verbatim>\<open>Isa_DOF\<close> is the abstract name of the text-file, \<^verbatim>\<open>Main\<close> etc. refer to imported
+  text files (recall that the import relation must be acyclic). \<^emph>\<open>keyword\<close>s are used to separate 
+  commands form each other;
+  predefined commands allow for the dynamic creation of new commands similarly 
+  to the definition of new functions in an interpreter shell (or: toplevel, see above.).
+  A command starts with a pre-declared keyword and specific syntax of this command;
+  the declaration of a keyword is only allowed in the same \<^verbatim>\<open>.thy\<close>-file where the
+  the corresponding new command is defined. The semantics of the command is expressed
+  in ML and consists of a @{ML_type "Toplevel.transition -> Toplevel.transition"}
+  function. Thus, the Isar-toplevel supports the generic document model 
+  and allows for user-programmed extensions.\<close>
 
 text\<open>In the traditional literature, Isabelle \<^verbatim>\<open>.thy\<close>-files were 
-were said to be processed by processed by two types of parsers:
+  were said to be processed by processed by two types of parsers:
 \<^enum> the "outer-syntax" (i.e. the syntax for commands) is processed 
   by a lexer-library and parser combinators built on top, and
 \<^enum> the "inner-syntax" (i.e. the syntax for @{term \<open>\<Lambda>\<close>} - terms) 
@@ -1169,13 +1134,12 @@ text\<open>This picture is less and less true for a number of reasons:
 
 section\<open>Basics: string, bstring and xstring\<close>
 text\<open>@{ML_type "string"} is the basic library type from the SML library
-in structure @{ML_structure "String"}. Many Isabelle operations produce
-or require formats thereof introduced as type synonyms 
-@{ML_type "bstring"} (defined in structure @{ML_structure "Binding"}
-and @{ML_type "xstring"} (defined in structure @{ML_structure "Name_Space"}.
-Unfortunately, the abstraction is not tight and combinations with 
-elementary routines might produce quite crappy results.
-\<close>
+  in structure @{ML_structure "String"}. Many Isabelle operations produce
+  or require formats thereof introduced as type synonyms 
+  @{ML_type "bstring"} (defined in structure @{ML_structure "Binding"}
+  and @{ML_type "xstring"} (defined in structure @{ML_structure "Name_Space"}.
+  Unfortunately, the abstraction is not tight and combinations with 
+  elementary routines might produce quite crappy results.\<close>
 
 ML\<open>val b = Binding.name_of@{binding "here"}\<close>
 text\<open>... produces the system output \verb+val it = "here": bstring+,
@@ -1200,36 +1164,35 @@ ML\<open> fun dark_matter x = XML.content_of (YXML.parse_body x)\<close>
 
 section\<open>Positions\<close>
 text\<open>A basic data-structure relevant for PIDE are \<^emph>\<open>positions\<close>; beyond the usual line- and column
-information they can represent ranges, list of ranges, and the name of the atomic sub-document
-in which they are contained. In the command:\<close>
+  information they can represent ranges, list of ranges, and the name of the atomic sub-document
+  in which they are contained. In the command:\<close>
 ML\<open>
 val pos = @{here};
 val markup = Position.here pos;
-writeln ("And a link to the declaration of 'here' is "^markup)
-\<close> 
+writeln ("And a link to the declaration of 'here' is "^markup)\<close> 
+
 (* \<^here>  *)
 text\<open> ... uses the antiquotation @{ML "@{here}"} to infer from the system lexer the actual position
-of itself in the global document, converts it to markup (a string-representation of it) and sends
-it via the usual @{ML "writeln"} to the interface. \<close>
+  of itself in the global document, converts it to markup (a string-representation of it) and sends
+  it via the usual @{ML "writeln"} to the interface. \<close>
 
 figure*[hyplinkout::figure,relative_width="40",src="''figures/markup-demo''"]
 \<open>Output with hyperlinked position.\<close>
 
 text\<open>@{docitem \<open>hyplinkout\<close>} shows the produced output where the little house-like symbol in the 
-display is hyperlinked to the position of @{ML "@{here}"} in the ML sample above.\<close>
+  display is hyperlinked to the position of @{ML "@{here}"} in the ML sample above.\<close>
 
 section\<open>Markup and Low-level Markup Reporting\<close>
 text\<open>The structures @{ML_structure Markup} and @{ML_structure Properties} represent the basic 
-annotation data which is part of the protocol sent from Isabelle to the front-end.
-They are qualified as "quasi-abstract", which means they are intended to be an abstraction of 
-the serialized, textual presentation of the protocol. Markups are structurally a pair of a key
-and properties; @{ML_structure Markup} provides a number of of such \<^emph>\<open>key\<close>s for annotation classes
-such as "constant", "fixed", "cartouche", some of them quite obscure. Here is a code sample
-from \<^theory_text>\<open>Isabelle_DOF\<close>. A markup must be tagged with an id; this is done by the @{ML serial}-function
-discussed earlier. Markup Operations, were used for hyperlinking applications to binding
-occurrences, info for hovering, infors for type ... \<close>  
+  annotation data which is part of the protocol sent from Isabelle to the front-end.
+  They are qualified as "quasi-abstract", which means they are intended to be an abstraction of 
+  the serialized, textual presentation of the protocol. Markups are structurally a pair of a key
+  and properties; @{ML_structure Markup} provides a number of of such \<^emph>\<open>key\<close>s for annotation classes
+  such as "constant", "fixed", "cartouche", some of them quite obscure. Here is a code sample
+  from \<^theory_text>\<open>Isabelle_DOF\<close>. A markup must be tagged with an id; this is done by the @{ML serial}-function
+  discussed earlier. Markup Operations, were used for hyperlinking applications to binding
+  occurrences, info for hovering, infors for type ... \<close>  
 ML\<open>
-
 (* Position.report is also a type consisting of a pair of a position and markup. *)
 (* It would solve all my problems if I find a way to infer the defining Position.report
    from a type definition occurence ... *)
@@ -1254,7 +1217,6 @@ Markup.theoryN : string;
 serial();   (* A global, lock-guarded seriel counter used to produce unique identifiers,
                be it on the level of thy-internal states or as reference in markup in
                PIDE *)
-
 \<close>
 
 
@@ -1283,8 +1245,8 @@ end
 \<close>
 
 text\<open>The @\<open>ML report_defining_occurrence\<close>-function above takes a position and a "cid" parsed
-in the Front-End, converts this into markup together with a unique number identifying this
-markup, and sends this as a report to the Front-End. \<close>
+  in the Front-End, converts this into markup together with a unique number identifying this
+  markup, and sends this as a report to the Front-End. \<close>
 
 
 subsection\<open>A Slightly more Complex Example\<close>
@@ -1369,25 +1331,23 @@ text\<open>The pudding comes with the eating: \<close>
 subsection\<open>Environment Structured Reporting\<close>
 
 text\<open> The structure @{ML_structure \<open>Name_Space\<close>} offers an own infra-structure for names and
-manages the markup accordingly.  MORE TO COME\<close>
+      manages the markup accordingly.  MORE TO COME\<close>
 text\<open> @{ML_type "'a Name_Space.table"} \<close>
 
 
 section\<open> The System Lexer and Token Issues\<close>
 text\<open>Four syntactic contexts are predefined in Isabelle (others can be added): 
-the ML context, the text context, the Isar-command context and the teerm-context, referring
-to different needs of the Isabelle Framework as an extensible framework supporting incremental,
-partially programmable extensions and as a Framework geared towards Formal Proofs and therefore
-mathematical notations. The basic data-structure for the lexical treatment of these  
-
-\<close>
+  the ML context, the text context, the Isar-command context and the teerm-context, referring
+  to different needs of the Isabelle Framework as an extensible framework supporting incremental,
+  partially programmable extensions and as a Framework geared towards Formal Proofs and therefore
+  mathematical notations. The basic data-structure for the lexical treatment of these elemens
+  are @{ML_structure "Token"}'s. \<close>
 
 subsection\<open>Tokens\<close>
 
 text\<open>The basic entity that lexers treat are \<^emph>\<open>tokens\<close>. defined in @{ML_structure "Token"}
-It provides a classification infrastructure, the references to positions and Markup 
-as well as way's to annotate tokens with (some) values they denote:
-\<close>
+  It provides a classification infrastructure, the references to positions and Markup 
+  as well as way's to annotate tokens with (some) values they denote:\<close>
 
 ML\<open>
 local
@@ -1444,20 +1404,20 @@ ML\<open>
 
 section\<open> Combinator Parsing \<close>  
 text\<open>Parsing Combinators go back to monadic programming as advocated by Wadler et. al, and has been 
-worked out @{cite "DBLP:journals/jfp/Hutton92"}. Parsing combinators are one of the two
-major parsing technologies of the Isabelle front-end, in particular for the outer-syntax used
-for the parsing of toplevel-commands. The core of the combinator library is 
-@{ML_structure \<open>Scan\<close>} providing the @{ML_type "'a parser"} which is a synonym for
-@{ML_type " Token.T list -> 'a * Token.T list"}. 
-
- "parsers" are actually  interpreters; an 'a parser is a function that parses
-an input stream and computes(=evaluates, computes) it into 'a. 
-Since the semantics of an Isabelle command is a transition => transition 
-or theory $\Rightarrow$ theory  function, i.e. a global system transition.
-parsers of that type can be constructed and be bound as call-back functions
-to a table in the Toplevel-structure of Isar.
-
-The library also provides a bunch of infix parsing combinators, notably:\<close>
+  worked out @{cite "DBLP:journals/jfp/Hutton92"}. Parsing combinators are one of the two
+  major parsing technologies of the Isabelle front-end, in particular for the outer-syntax used
+  for the parsing of toplevel-commands. The core of the combinator library is 
+  @{ML_structure \<open>Scan\<close>} providing the @{ML_type "'a parser"} which is a synonym for
+  @{ML_type " Token.T list -> 'a * Token.T list"}. 
+  
+   "parsers" are actually  interpreters; an 'a parser is a function that parses
+  an input stream and computes(=evaluates, computes) it into 'a. 
+  Since the semantics of an Isabelle command is a transition => transition 
+  or theory $\Rightarrow$ theory  function, i.e. a global system transition.
+  parsers of that type can be constructed and be bound as call-back functions
+  to a table in the Toplevel-structure of Isar.
+  
+  The library also provides a bunch of infix parsing combinators, notably:\<close>
 
 ML\<open>
   val _ = op !! : ('a * message option -> message) -> ('a -> 'b) -> 'a -> 'b
@@ -1502,9 +1462,9 @@ val _ = Scan.lift Args.cartouche_input : Input.source context_parser;\<close>
 subsection\<open>Advanced Parser Library\<close>
 
 text\<open>There are two parts. A general multi-purpose parsing combinator library is 
-found under @{ML_structure "Parse"}, providing basic functionality for parsing strings
-or integers. There is also an important combinator that reads the current position information
-out of the input stream:\<close>
+  found under @{ML_structure "Parse"}, providing basic functionality for parsing strings
+  or integers. There is also an important combinator that reads the current position information
+  out of the input stream:\<close>
 ML\<open>
 Parse.nat: int parser;  
 Parse.int: int parser;
@@ -1521,12 +1481,11 @@ Parse.position Args.cartouche_input;
 \<close>
 
 text\<open>The second part is much more high-level, and can be found under @{ML_structure Args}.
-In parts, these combinators are again based on more low-level combinators, in parts they serve as 
-an an interface to the underlying Earley-parser for mathematical notation used in types and terms.
-This is perhaps meant with the fairly cryptic comment:
-"Quasi-inner syntax based on outer tokens: concrete argument syntax of
-attributes, methods etc." at the beginning of this structure.
-\<close>
+  In parts, these combinators are again based on more low-level combinators, in parts they serve as 
+  an an interface to the underlying Earley-parser for mathematical notation used in types and terms.
+  This is perhaps meant with the fairly cryptic comment:
+  "Quasi-inner syntax based on outer tokens: concrete argument syntax of
+  attributes, methods etc." at the beginning of this structure.\<close>
 
 ML\<open>
 
@@ -1608,11 +1567,11 @@ in val _ = () end
 subsection\<open> Bindings \<close>  
 
 text\<open> The structure @{ML_structure "Binding"} serves as 
-\<open>structured name bindings\<close>, as says the description, i.e. a mechanism to basically 
-associate an input string-fragment to its position. This concept is vital in all parsing processes
-and the interaction with PIDE.
+  \<open>structured name bindings\<close>, as says the description, i.e. a mechanism to basically 
+  associate an input string-fragment to its position. This concept is vital in all parsing processes
+  and the interaction with PIDE.
 
-Key are two things:
+  Key are two things:
 \<^enum> the type-synonym @{ML_type "bstring"} which is synonym to @{ML_type "string"}
   and intended for "primitive names to be bound"
 \<^enum> the projection @{ML "Binding.pos_of :  binding -> Position.T"} 
@@ -1655,8 +1614,8 @@ ML\<open>
 section\<open>Term Parsing\<close>  
 
 text\<open>The heart of the parsers for mathematical notation, based on an Earley parser that can cope
-with incremental changes of the grammar as required for sophisticated mathematical output, is hidden
-behind the API described in this section.\<close>
+  with incremental changes of the grammar as required for sophisticated mathematical output, is hidden
+  behind the API described in this section.\<close>
   
 text\<open> Note that the naming underlies the following convention : 
    there are:
@@ -1792,16 +1751,16 @@ text\<open>It provides a number of hooks that can be used for redirection hacks 
 
 section \<open> Output: LaTeX \<close>
 text\<open>The heart of the LaTeX generator is to be found in the structure @{ML_structure Thy_Output}.
-This is an own parsing and writing process, with the risc that a parsed file in the IDE parsing
-process can not be parsed for the LaTeX Generator. The reason is twofold:
+  This is an own parsing and writing process, with the risc that a parsed file in the IDE parsing
+  process can not be parsed for the LaTeX Generator. The reason is twofold:
 \<^enum> The LaTeX Generator makes a rough attempt to mimic the LayOut if the thy-file; thus, its
   spacing is relevant.
 \<^enum> there is a special bracket \<open>(*<*)\<close> ... \<open>(*>*)\<close> that allows to specify input that is checked by
   Isabelle, but excluded from the LaTeX generator (this is handled in an own sub-parser
   called @{ML "Document_Source.improper"} where also other forms of comment parsers are provided.
 
-Since Isabelle2018, an own AST is provided for the LaTeX syntax, analogously to 
-@{ML_structure "Pretty"}. Key functions of this structure @{ML_structure "Latex"} are:
+  Since Isabelle2018, an own AST is provided for the LaTeX syntax, analogously to 
+  @{ML_structure "Pretty"}. Key functions of this structure @{ML_structure "Latex"} are:
 \<close>
 
 ML\<open>
@@ -1927,16 +1886,15 @@ As one can see, check-routines internally generate the markup.
 
 section*[cartouches::technical]\<open>Inner Syntax Cartouches\<close>
 text\<open> The cascade-syntax principle underlying recent isabelle versions requires a 
-particular mechanism, called "cartouche" by Makarius who was influenced by French 
-Wine and French culture when designing this.
+  particular mechanism, called "cartouche" by Makarius who was influenced by French 
+  Wine and French culture when designing this.
 
-When parsing terms or types (via the Earley Parser), a standard mechanism for
-calling another parser inside the current process is needed that is bound to the 
-\<open>(\<open>)\<close> ... \<open>(\<close>)\<close> paranthesis'. 
-\<close>
+  When parsing terms or types (via the Earley Parser), a standard mechanism for
+  calling another parser inside the current process is needed that is bound to the 
+  \<open>(\<open>)\<close> ... \<open>(\<close>)\<close> paranthesis'. \<close>
 
 text\<open>The following example --- drawn from the Isabelle/DOF implementation --- allows
-to parse UTF8 - Unicode strings as alternative to @{term "''abc''"} HOL-strings.\<close>
+  to parse UTF8 - Unicode strings as alternative to @{term "''abc''"} HOL-strings.\<close>
 
 ML\<open>\<comment> \<open>Dynamic setup of inner syntax cartouche\<close>
 
@@ -2000,13 +1958,13 @@ fun parse_translation_cartouche binding l f_integer accu =
 \<close>
 
 text\<open>The following registration of this cartouche for strings is fails because it has
- already been done in the surrounding Isabelle/DOF environment... \<close>
-(*
-parse_translation \<open>
-  [( @{syntax_const "_cartouche_string"}
-   , parse_translation_cartouche \<^binding>\<open>cartouche_type\<close> Cartouche_Grammar.default (K I) ())]
-\<close>
-*)
+  already been done in the surrounding Isabelle/DOF environment... \<close>
+  (*
+  parse_translation \<open>
+    [( @{syntax_const "_cartouche_string"}
+     , parse_translation_cartouche \<^binding>\<open>cartouche_type\<close> Cartouche_Grammar.default (K I) ())]
+  \<close>
+  *)
 
 (* test for this cartouche... *) 
 term  "\<open>A \<Longrightarrow> B\<close> = ''''"
@@ -2015,22 +1973,22 @@ term  "\<open>A \<Longrightarrow> B\<close> = ''''"
 
 chapter*[c::conclusion]\<open>Conclusion\<close>
 text\<open> This interactive Isabelle Programming Cook-Book represents my current way 
-to view and explain Isabelle programming API's to students and collaborators. 
-It differs from the reference  manual in some places on purpose, since I believe 
-that a lot of internal Isabelle API's need a more conceptual view on what is happening 
-(even if this conceptual view is at times over-abstracting a little).
-It also offers a deliberately different abstraction  to the explanations in form of comments
-in the sources or in the Reference Manual.
-
-The descriptions of some sources may appear lengthy and repetitive and redundant - but this kind 
-of repetition not only give an idea of the chosen abstraction levels on some interfaces, but also
-represents --- since this is a "living document" (a notion I owe Simon Foster) --- a continuous check
-for each port of our material to  each more recent Isabelle version, where the first attempts
-to load it will fail, but give another source of information over the modifications of
-the system interface for parts relevant to our own development work.
-
-All hints and contributions of collegues and collaborators are greatly welcomed; all errors
-and the roughness of this presentation is entirely my fault.
+  to view and explain Isabelle programming API's to students and collaborators. 
+  It differs from the reference  manual in some places on purpose, since I believe 
+  that a lot of internal Isabelle API's need a more conceptual view on what is happening 
+  (even if this conceptual view is at times over-abstracting a little).
+  It also offers a deliberately different abstraction  to the explanations in form of comments
+  in the sources or in the Reference Manual.
+  
+  The descriptions of some sources may appear lengthy and repetitive and redundant - but this kind 
+  of repetition not only give an idea of the chosen abstraction levels on some interfaces, but also
+  represents --- since this is a "living document" (a notion I owe Simon Foster) --- a continuous check
+  for each port of our material to  each more recent Isabelle version, where the first attempts
+  to load it will fail, but give another source of information over the modifications of
+  the system interface for parts relevant to our own development work.
+  
+  All hints and contributions of collegues and collaborators are greatly welcomed; all errors
+  and the roughness of this presentation is entirely my fault.
 \<close>
 (*<*)
 
